A call-free branch for experimentation.

ADT.v
@@ -8,98 +8,53 @@ Local Open Scope type_scope.
 
 (** * Basic ADT definitions *)
 (** Type of a context *)
-Definition Build_ADTContext
-           (rep mutIdx obsIdx : Type)
-           (mutDom : mutIdx -> Type)
-           (obsDom obsCod : obsIdx -> Type): Context :=
-  {| names := mutIdx + obsIdx;
-     dom idx := rep *
-                match idx with
-                  | inl mIdx => mutDom mIdx
-                  | inr oIdx => obsDom oIdx
-                end;
-     cod idx := match idx with
-                  | inl mIdx => rep
-                  | inr oIdx => obsCod oIdx
-                end |}.
 
-(** Type of a mutator method *)
-Definition mutatorMethodTypeUnbundled (Ty mutIdx obsIdx dom : Type)
-           (mutDom : mutIdx -> Type)
-           (obsDom obsCod : obsIdx -> Type)
-           (* we give a [Context] here so typeclass resolution can pick it up *)
-           (ctx := Build_ADTContext Ty mutDom obsDom obsCod)
+(** Type of a mutator method. *)
+Definition mutatorMethodType (Ty dom : Type)
   := Ty    (* Initial model *)
      -> dom (* Actual argument*)
      -> Comp Ty (* Final Model *).
 
-(** Type of an obeserver method *)
-Definition observerMethodTypeUnbundled (Ty mutIdx obsIdx dom cod : Type)
-           (mutDom : mutIdx -> Type)
-           (obsDom obsCod : obsIdx -> Type)
-           (* we give a [Context] here so typeclass resolution can pick it up *)
-           (ctx := Build_ADTContext Ty mutDom obsDom obsCod)
+(** Type of an obeserver method. *)
+Definition observerMethodType (Ty dom cod : Type)
   := Ty    (* Initial model *)
      -> dom (* Actual argument*)
      -> Comp cod. (* Return value *)
 
-(** Type of a mutator method bundled with its context *)
-Definition mutatorMethodType (Ty dom : Type)
-  := Ty    (* Initial model *)
-     -> dom (* Actual argument*)
-     -> BundledComp Ty (* Final Model *).
+Record ADTSig :=
+  { MutatorIndex : Type;
+     (** The index set of mutators *)
 
-(** Type of an obeserver method *)
-Definition observerMethodType (Ty dom cod : Type)
-  := Ty    (* Initial model *)
-     -> dom (* Actual argument*)
-     -> BundledComp cod. (* Return value *)
+     ObserverIndex : Type;
+     (** The index set of observers *)
+
+     MutatorDom : MutatorIndex -> Type;
+     (** The representation-independent piece of the
+         domain of mutator methods. **)
+
+    ObserverDom : ObserverIndex -> Type;
+     (** The representation-independent piece of the
+         domain of observer methods. **)
+
+    ObserverCod : ObserverIndex -> Type
+     (** The codomain of observer methods. **)
+
+  }.
 
 (** Interface of an ADT *)
-Record ADT :=
+Record ADT (Sig : ADTSig) :=
   {
     Rep : Type;
     (** The representation type of the ADT **)
 
-    MutatorIndex : Type;
-    (** The index set of mutators *)
-
-    ObserverIndex : Type;
-    (** The index set of observers *)
-
-    MutatorDom : MutatorIndex -> Type;
-
-    ObserverDom : ObserverIndex -> Type;
-
-    ObserverCod : ObserverIndex -> Type;
-
-    UnbundledMutatorMethods :
-      forall idx : MutatorIndex,
-        mutatorMethodTypeUnbundled Rep (MutatorDom idx)
-                                   MutatorDom ObserverDom ObserverCod;
+    MutatorMethods :
+      forall idx : MutatorIndex Sig,
+        mutatorMethodType Rep (MutatorDom Sig idx);
     (** Mutator method implementations *)
 
-    UnbundledObserverMethods :
-      forall idx : ObserverIndex,
-        observerMethodTypeUnbundled Rep (ObserverDom idx) (ObserverCod idx)
-                                    MutatorDom ObserverDom ObserverCod
+    ObserverMethods :
+      forall idx : ObserverIndex Sig,
+        observerMethodType Rep (ObserverDom Sig idx) (ObserverCod Sig idx)
     (** Observer method implementations *)
 
   }.
-
-Definition ADTLookupContext (A : ADT) : LookupContext
-  := {| LContext := Build_ADTContext (Rep A) (MutatorDom A) (ObserverDom A) (ObserverCod A);
-        lookup idx := match idx with
-                        | inl mIdx => fun state_value =>
-                                        UnbundledMutatorMethods A mIdx (fst state_value) (snd state_value)
-                        | inr oIdx => fun state_value =>
-                                        UnbundledObserverMethods A oIdx (fst state_value) (snd state_value)
-                      end |}.
-
-Definition MutatorMethods (A : ADT) (i : MutatorIndex A)
-: mutatorMethodType (Rep A) (MutatorDom A i)
-  := fun m x => ``[ UnbundledMutatorMethods A i m x with ADTLookupContext A ]`` .
-
-Definition ObserverMethods (A : ADT) (i : ObserverIndex A)
-: observerMethodType (Rep A) (ObserverDom A i) (ObserverCod A i)
-  := fun m x => ``[ UnbundledObserverMethods A i m x with ADTLookupContext A ]``.
