ADTHide.v
@@ -1,0 +1,41 @@
+Require Import Common Computation ADT Ensembles.
+
+Section HideADT.
+
+  Context {extSig : ADTSig}.
+  (* The extended signature *)
+
+  Context {resMutatorIndex : Type}.
+  (* The restricted set of mutator indices *)
+
+  Context {resObserverIndex : Type}.
+  (* The restricted set of observer indices *)
+
+  Variable MutatorMap : resMutatorIndex -> MutatorIndex extSig.
+  (* Map from restricted to extended mutator indices *)
+
+  Variable ObserverMap : resObserverIndex -> ObserverIndex extSig.
+  (* Map from restricted to extended observer indices *)
+
+  Definition resSig :=
+    {| MutatorIndex := resMutatorIndex;
+       ObserverIndex := resObserverIndex;
+       MutatorDom idx := MutatorDom extSig (MutatorMap idx);
+       ObserverDom idx := ObserverDom extSig (ObserverMap idx);
+       ObserverCod idx := ObserverCod extSig (ObserverMap idx)
+    |}.
+  (* The signature of the ADT with restricted mutator and observer indices *)
+
+
+  Definition HideADT (extADT : ADT extSig) : ADT resSig :=
+    match extADT with
+        {| Rep := Rep;
+           MutatorMethods := extMutatorMethods;
+           ObserverMethods := extObserverMethods
+        |} =>
+        Build_ADT resSig
+          (fun idx => extMutatorMethods (MutatorMap idx))
+          (fun idx => extObserverMethods (ObserverMap idx))
+    end.
+
+End HideADT.
