ADTRefinement/RefineHideADT.v
@@ -1,0 +1,30 @@
+Require Import Common Computation ADT Ensembles ADTHide.
+Require Import ADTRefinement.Core.
+
+Add Parametric Morphism
+    extSig'
+    oldMutatorIndex oldObserverIndex
+    (MutatorMap : oldMutatorIndex -> MutatorIndex extSig')
+    (ObserverMap : oldObserverIndex -> ObserverIndex extSig')
+    oldADT
+: (fun newADT => refineADT oldADT (HideADT MutatorMap ObserverMap newADT))
+    with signature
+    refineADT ==> impl
+as RefineHideADT.
+Proof.
+  unfold impl.
+  intros; inversion H; inversion H0; subst;
+  unfold HideADT in *; destruct x; destruct y;
+  destruct oldADT; simpl in *.
+  econstructor 1 with
+  (SiR := fun r_o r_n =>
+            exists r_n', SiR0 r_o r_n' /\ SiR r_n' r_n);
+    simpl; intros.
+  - destruct_ex; intuition.
+    rewrite <- H1, <- H5; eauto.
+    autorewrite with refine_monad; f_equiv;
+    unfold pointwise_relation; intros.
+    econstructor; inversion_by computes_to_inv; eauto.
+  - destruct_ex; intuition.
+    rewrite <- H2, <- H6; eauto; reflexivity.
+Qed.
