ADTRefinement/Specs.v
@@ -1,15 +1,20 @@
 Set Implicit Arguments.
 
-(* Specification of mutator method. *)
-Definition mutatorMethodSpec (Ty : Type) :=
-  Ty    (* Initial model *)
-  -> nat (* Actual argument*)
-  -> Ty (* Final Model *)
-  -> Prop.
+Section ADTSpecs.
 
-(* Specification of an observer method *)
-Definition observerMethodSpec (Ty : Type) :=
-  Ty    (* Initial model *)
-  -> nat (* Actual argument*)
-  -> nat (* Return value *)
-  -> Prop.
+  (* Specification of mutator method. *)
+
+  Definition mutatorMethodSpec (Ty Dom : Type) :=
+    Ty    (* Initial model *)
+    -> Dom (* Actual argument*)
+    -> Ty (* Final Model *)
+    -> Prop.
+
+  (* Specification of an observer method *)
+  Definition observerMethodSpec (Ty Dom Cod : Type) :=
+    Ty    (* Initial model *)
+    -> Dom (* Actual argument*)
+    -> Cod (* Return value *)
+    -> Prop.
+
+End ADTSpecs.
