Computation/Refinements/General.v
@@ -22,224 +22,84 @@ Local Ltac t_refine :=
                | progress destruct_head_hnf and
                | progress specialize_all_ways ].
 
-Section structural.
-
-  (* BD: This defines a notion of equivalnce for call-free
-     computations. Computations which are call-free compute to
-     the same value regardless of the context, naturally. *)
-
-  Inductive refineBundled_structural {ctx1 ctx2 : LookupContext}
-  : forall A, @Comp ctx1 A -> @Comp ctx2 A -> Prop :=
-| rbEq_Return : forall A (x : A), refineBundled_structural (Return x) (Return x)
-| rbEq_Bind : forall A B c1 c2 f1 f2,
-                refineBundled_structural c1 c2
-                -> (forall v : A,
-                      computes_to (ctx := ctx1) c1 v
-                      -> computes_to (ctx := ctx2) c2 v
-                      -> refineBundled_structural (f1 v) (f2 v))
-                -> @refineBundled_structural _ _ B (Bind c1 f1) (Bind c2 f2)
-| rbEq_Pick : forall A P, @refineBundled_structural ctx1 ctx2 A (Pick P) (Pick P).
-
-
-  Lemma refineBundled_structural_impl_refineBundledEquiv {A} (c1 c2 : BundledComp A)
-  : refineBundled_structural c1 c2 -> refineBundledEquiv c1 c2.
-  Proof.
-    destruct c1 as [ctx1 c1], c2 as [ctx2 c2]; simpl.
-    induction 1; t_refine.
-  Qed.
-End structural.
-
-Ltac refineBundledEquiv_reflexivity_ignore_context :=
-  apply refineBundled_structural_impl_refineBundledEquiv;
-  simpl;
-  repeat (econstructor || intro).
-
-Ltac equate_evar_context :=
-  unfold refineBundledEquiv, refineBundled; simpl;
-  lazymatch goal with
-    | [ |- @refineEquiv ?A ?ctx1 (@CompContext ?B ?e) ?v1 ?v2 ]
-      => is_evar e; refine (_ : @refineEquiv A ctx1 (@CompContext B {| CompContext := ctx1 |}) v1 v2)
-    | [ |- @refine ?A ?ctx1 (@CompContext ?B ?e) ?v1 ?v2 ]
-      => is_evar e; refine (_ : @refine A ctx1 (@CompContext B {| CompContext := ctx1 |}) v1 v2)
-  end;
-  simpl.
-
-Ltac etransitivity_context :=
-  etransitivity;
-  [ equate_evar_context | refineBundledEquiv_reflexivity_ignore_context ].
-
 Section general_refine_lemmas.
-  Lemma refineEquiv_is_computational {A} {ctx1 ctx2 : LookupContext} {c} (CompC : @is_computational ctx1 A c)
-  : @refineEquiv _ ctx1 ctx2
-                c (ret (is_computational_val CompC)).
+  
+  Lemma refineEquiv_is_computational {A} {c} (CompC : @is_computational A c)
+  : @refineEquiv _ c (ret (is_computational_val CompC)).
   Proof.
     unfold refineEquiv, refine.
     pose proof (is_computational_val_computes_to CompC).
     t_refine.
   Qed.
 
-  Definition refineBundledEquiv_is_computational A {ctx1 : LookupContext} (c : BundledComp A)
-  : forall (CompC : is_computational c),
-      refineBundledEquiv c ``[ ret (is_computational_val CompC) with ctx1 ]``
-    := @refineEquiv_is_computational A _ ctx1 c.
-
-  Lemma refine_pick A {ctx1 ctx2 : LookupContext}
-        (P : A -> Prop) c (H : forall x, c ↝ x -> P x)
-  : @refine A ctx1 ctx2
-            { x : A | P x }%comp
+  Lemma refine_pick A (P : A -> Prop) c (H : forall x, c ↝ x -> P x)
+  : @refine A ({x : A | P x })%comp
             c.
   Proof. t_refine. Qed.
 
-  Definition refineBundled_pick A {ctx1 : LookupContext}
-             P (c : BundledComp A)
-  : _ -> refineBundled ``[ { x : A | P x }%comp with ctx1 ]``
-                       c
-    := @refine_pick _ _ _ P c.
-
-  Lemma refine_pick_pick A {ctx1 ctx2 : LookupContext} (P1 P2 : A -> Prop)
+  Lemma refine_pick_pick A (P1 P2 : A -> Prop)
         (H : forall x, P2 x -> P1 x)
-  : @refine _ ctx1 ctx2
+  : @refine _
             { x : A | P1 x }%comp
             { x : A | P2 x }%comp.
   Proof. t_refine. Qed.
 
-  Definition refineBundled_pick_pick
-  : forall A {ctx1 ctx2} P1 P2 H,
-      refineBundled ``[ _ with ctx1 ]``
-                    ``[ _ with ctx2 ]``
-    := refine_pick_pick.
-
-  Lemma refineEquiv_pick_pick A {ctx1 ctx2} (P1 P2 : A -> Prop)
+  Lemma refineEquiv_pick_pick A (P1 P2 : A -> Prop)
         (H : forall x, P1 x <-> P2 x)
-  : @refineEquiv _ ctx1 ctx2
+  : @refineEquiv _
                  { x : A | P1 x }%comp
                  { x : A | P2 x }%comp.
   Proof. t_refine. Qed.
 
-  Definition refineBundledEquiv_pick_pick
-  : forall A {ctx1 ctx2} P1 P2 H,
-      refineBundledEquiv ``[ _ with ctx1 ]``
-                         ``[ _ with ctx2 ]``
-    := refineEquiv_pick_pick.
-
-  Lemma refineEquiv_pick_pair {ctx1 ctx2} A B (PA : A -> Prop) (PB : B -> Prop)
-  : @refineEquiv _ ctx1 ctx2
+  Lemma refineEquiv_pick_pair A B (PA : A -> Prop) (PB : B -> Prop)
+  : @refineEquiv _
                  { x : A * B | PA (fst x) /\ PB (snd x) }%comp
                  (a <- { a : A | PA a };
                   b <- { b : B | PB b };
                   ret (a, b))%comp.
   Proof. t_refine. Qed.
 
-  Definition refineEquivBundled_pick_pair
-  : forall A {ctx1 ctx2} P1 P2 H,
-      refineBundledEquiv ``[ _ with ctx1 ]``
-                         ``[ _ with ctx2 ]``
-    := refineEquiv_pick_pick.
-
-  Definition refineEquiv_split_ex {ctx1 ctx2} A B (P : A -> Prop) (P' : A -> B -> Prop)
-  : @refineEquiv _ ctx1 ctx2
+  Definition refineEquiv_split_ex A B
+             (P : A -> Prop) (P' : A -> B -> Prop)
+  : @refineEquiv _ 
                  { b | exists a, P a /\ P' a b }%comp
                  (a <- { a | P a /\ exists b, P' a b };
                   { b | P' a b })%comp.
   Proof. t_refine. Qed.
 
-  Definition refineBundledEquiv_split_ex
-  : forall {ctx1 ctx2} A B P P',
-      refineBundledEquiv `[ _ ]` `[ _ ]`
-    := @refineEquiv_split_ex.
-
-  Definition refineEquiv_pick_contr_ret {ctx1 ctx2} A (P : A -> Prop)
+  Definition refineEquiv_pick_contr_ret A (P : A -> Prop)
              (x : A) (H : unique P x)
-  : @refineEquiv _ ctx1 ctx2
+  : @refineEquiv _ 
                  { y | P y }
                  (ret x).
   Proof. t_refine. Qed.
 
-  Definition refineEquiv_pick_eq {ctx1 ctx2}
+  Definition refineEquiv_pick_eq 
              A (x : A)
-  : @refineEquiv _ ctx1 ctx2
+  : @refineEquiv _ 
                  { y | y = x }%comp
                  (ret x).
   Proof. t_refine. Qed.
 
-  Definition refineBundledEquiv_pick_eq
-  : forall {ctx1 ctx2}
-           A (x : A),
-      refineBundledEquiv `[ _ ]` `[ _ ]`
-    := @refineEquiv_pick_eq.
-
-  Definition refineEquiv_pick_eq' {ctx1 ctx2}
-             A (x : A)
-  : @refineEquiv _ ctx1 ctx2
-                 { y | x = y }%comp
+  Definition refineEquiv_pick_eq' A (x : A)
+  : @refineEquiv _ { y | x = y }%comp
                  (ret x).
   Proof. t_refine. Qed.
 
-  Definition refineBundledEquiv_pick_eq'
-  : forall {ctx1 ctx2}
-           A (x : A),
-      refineBundledEquiv `[ _ ]` `[ _ ]`
-    := @refineEquiv_pick_eq'.
-
-  Definition refineBundledEquiv_split_func_ex {ctx1 ctx2}
-             A B (P : A -> Prop) (f : A -> B)
-  : refineBundledEquiv ``[ { b | exists a, P a /\ b = f a}%comp with ctx1 ]``
-                       ``[ (a <- { a | P a};
-                            ret (f a))%comp
-                           with ctx2 ]``.
-  Proof.
-    repeat setoid_rewrite refineBundledEquiv_split_ex.
-    (** I want to just [setoid_rewrite refineBundledEquiv_pick_eq].  But I can't because things don't line up nicely, and there are no parameterized setoid relations.  :-(  So instead we need to [etransitivity_context] instead. *)
-    etransitivity_context.
-    setoid_rewrite refineEquiv_pick_eq.
-    (** [erewrite] is buggy: https://coq.inria.fr/bugs/show_bug.cgi?id=3244 *)
-    erewrite (@refineEquiv_pick_pick _ _ _).
-    - reflexivity.
-    - abstract (repeat (intro || esplit); intuition).
-  Qed.
-
-  Definition refineEquiv_split_func_ex {ctx1 ctx2}
+  Definition refineEquiv_split_func_ex
   : forall A B (P : A -> Prop) (f : A -> B),
-      @refineEquiv _ ctx1 ctx2
-                   { b | exists a, P a /\ b = f a}%comp
+      @refineEquiv _ { b | exists a, P a /\ b = f a}%comp
                    (a <- { a | P a};
-                    ret (f a))%comp
-    := refineBundledEquiv_split_func_ex.
+                    ret (f a))%comp.
+  Proof. t_refine. Qed.
 
-  Definition refineBundledEquiv_split_func_ex2 {ctx1 ctx2} A A' B (P : A -> Prop) (P' : A' -> Prop)
+  Definition refineEquiv_split_func_ex2 
+             A A' B (P : A -> Prop) (P' : A' -> Prop)
              (f : A -> A' -> B)
-  : refineBundledEquiv ``[ { b | exists a, P a /\ exists a', P' a' /\ b = f a a'} with ctx1 ]``
-                       ``[ (a <- { a | P a};
-                            a' <- { a' | P' a'};
-                            ret (f a a'))
-                           with ctx2 ]``.
-  Proof.
-    etransitivity_context.
-    (** >:-(   We shouldn't need to clear the context to get typeclass resolution and setoid rewriting to work. *)
-    clear.
-    repeat setoid_rewrite (@refineEquiv_split_ex _ _).
-    setoid_rewrite (@refineEquiv_pick_eq _ _).
-    split; intro; intros;
-    inversion_by computes_to_inv; subst;
-    repeat econstructor; eassumption.
-  Qed.
-
-  Definition refineEquiv_split_func_ex2 {ctx1 ctx2}
-  : forall A A' B (P : A -> Prop) (P' : A' -> Prop)
-           (f : A -> A' -> B),
-      refineEquiv _ _
-    := @refineBundledEquiv_split_func_ex2 ctx1 ctx2.
-
-  (* [refine_bind] assumes a uniform context, which we don't always have.*)
-  Definition refineBundled_bind {ctx1 ctx2 : LookupContext}
-  : forall A B a a' (b : A -> @Comp ctx1 B) (b' : A -> @Comp ctx2 B),
-      refineBundled ``[a with ctx1]`` ``[a' with ctx2]``
-      -> (forall a, refineBundled ``[b a with ctx1]`` ``[b' a with ctx2]``)
-      -> refineBundled ``[(a'' <- a; b a'') with ctx1]`` ``[a'' <- a'; b' a'' with ctx2]`` .
-  Proof.
-    unfold refineBundled, refine; intros.
-    apply_in_hyp computes_to_inv; simpl in *; destruct_ex; intuition;
-    econstructor; eauto.
-  Qed.
+  : refineEquiv { b | exists a, P a /\ exists a', P' a' /\ b = f a a'}
+                (a <- { a | P a};
+                 a' <- { a' | P' a'};
+                 ret (f a a')).
+  Proof. t_refine. Qed.
 
 End general_refine_lemmas.
