Computation/SetoidMorphisms.v
@@ -4,71 +4,43 @@ Require Import Computation.Core.
 (** General Lemmas about the parametric morphism behavior of
     [computes_to], [refine], and [refineEquiv]. *)
 
-Add Parametric Relation A `{LookupContext}
-: (Comp A) (@refine A _ _)
+Add Parametric Relation A
+: (Comp A) (@refine A)
   reflexivity proved by reflexivity
   transitivity proved by transitivity
     as refine_rel.
 
 Add Parametric Relation A
-: (BundledComp A) (@refineBundled A)
-  reflexivity proved by reflexivity
-  transitivity proved by transitivity
-    as refineBundled_rel.
-
-Add Parametric Relation A `{LookupContext}
-: (Comp A) (@refineEquiv A _ _)
+: (Comp A) (@refineEquiv A)
   reflexivity proved by reflexivity
   symmetry proved by symmetry
   transitivity proved by transitivity
     as refineEquiv_rel.
 
-Add Parametric Relation A
-: (BundledComp A) (@refineBundledEquiv A)
-  reflexivity proved by reflexivity
-  symmetry proved by symmetry
-  transitivity proved by transitivity
-    as refineBundledEquiv_rel.
-
 Local Ltac t := unfold impl; intros; repeat (eapply_hyp || etransitivity).
 
-Add Parametric Morphism A `{LookupContext}
-: (@refine A _ _)
+Add Parametric Morphism A
+: (@refine A)
   with signature
-  (@refine A _ _) --> (@refine A _ _) ++> impl
+  (@refine A) --> (@refine A) ++> impl
     as refine_refine.
 Proof. t. Qed.
 
-Add Parametric Morphism A `{LookupContext}
-: (@refine A _ _)
+Add Parametric Morphism A 
+: (@refine A)
   with signature
-  (@refineEquiv A _ _) --> (@refineEquiv A _ _) ++> impl
+  (@refineEquiv A) --> (@refineEquiv A) ++> impl
     as refine_refineEquiv.
-Proof. t. Qed.
-
-
-Add Parametric Morphism A
-: (@refineBundled A)
-  with signature
-  (@refineBundled A) --> (@refineBundled A) ++> impl
-    as refineBundled_refineBundled.
-Proof. t. Qed.
-
-Add Parametric Morphism A
-: (@refineBundled A)
-  with signature
-  (@refineBundledEquiv A) --> (@refineBundledEquiv A) ++> impl
-    as refineBundled_refineBundledEquiv.
 Proof. t. Qed.
 
 Hint Constructors computes_to.
 
-Add Parametric Morphism `{LookupContext} A B
-: (@Bind _ A B)
+Add Parametric Morphism A B
+: (@Bind A B)
     with signature
-    (@refine A _ _)
-      ==> (pointwise_relation _ (@refine B _ _))
-      ==> (@refine B _ _)
+    (@refine A)
+      ==> (pointwise_relation _ (@refine B))
+      ==> (@refine B)
       as refine_bind.
 Proof.
   simpl; intros.
@@ -78,12 +50,12 @@ Proof.
   eauto.
 Qed.
 
-Add Parametric Morphism `{LookupContext} A B
-: (@Bind _ A B)
+Add Parametric Morphism A B
+: (@Bind A B)
     with signature
-    (@refineEquiv A _ _)
-      ==> (pointwise_relation _ (@refineEquiv B _ _))
-      ==> (@refineEquiv B _ _)
+    (@refineEquiv A)
+      ==> (pointwise_relation _ (@refineEquiv B))
+      ==> (@refineEquiv B)
       as refineEquiv_bind.
 Proof.
   idtac.
@@ -94,19 +66,3 @@ Proof.
   inversion_by computes_to_inv;
   eauto.
 Qed.
-
-(*Add Parametric Morphism `{LookupContext} A B
-: (@Bind names dom cod A B)
-    with signature
-    (@refineEquiv A names dom cod names dom cod lookup lookup)
-      ==> (pointwise_relation _ (@refineEquiv B names dom cod names dom cod lookup lookup))
-      ==> (@refine B names dom cod names dom cod lookup lookup)
-      as refineEquiv_refine_bind.
-Proof.
-  intros.
-  refine (proj1 (_ : refineEquiv _ _ _ _)).
-  simpl in *.
-  setoid_rewrite <- H.
-  setoid_rewrite_hyp.
-  reflexivity.
-Qed.*)
